Add literals set and continue minterms def

Test_Formulae.thy
@@ -221,6 +221,9 @@ typedef ('var, 'k::finite) literal
   = "{f::('var, 'k) sl_formula. f \<in> test_formulae} \<union> {(not f)|f. f \<in> test_formulae}"
   using test_formulae.intros(3) by force
 
+definition literals :: "('var, 'k::finite) sl_formula set"
+  where "literals = ({f::('var, 'k) sl_formula. f \<in> test_formulae} \<union> {(not f)|f. f \<in> test_formulae})"
+
 definition to_sl_formula :: "('var, 'k::finite) literal \<Rightarrow> ('var, 'k) sl_formula"
   where "to_sl_formula f = Rep_literal f"
 
@@ -231,11 +234,10 @@ subsubsection {* Useful Literals Results *}
 
 lemma to_sl_formula_to_literal:
   fixes f::"('var, 'k::finite) sl_formula"
-  assumes "(f \<in> test_formulae) \<or> ((not f) \<in> test_formulae)"
+  assumes "f \<in> literals"
   shows "equivalence (UNIV::'addr set) (to_sl_formula (to_literal f)) f"
-proof -
-
-  oops
+  using literals_def by (metis (mono_tags) Abs_literal_inverse assms equivalence_def 
+                         logical_consequence_def to_literal_def to_sl_formula_def)
 
 
 end
